#  Regra do Produto
## Ex. 1 
$$f(x) = x^-1\cdot e^x$$

	$$f'(x) = -x^-2 \cdot e^x + x^-1 \cdot e^x$$
	$$f'(x) = -\frac{e^x}{x^2} + \frac{e^x}{x}$$
	$$f'(x) = -\frac{e^x}{x^2} + \frac{x \cdot e^x}{x^2}$$
	$$f'(x) = \frac{-e^x + xe^x}{x^2}$$
## Ex. 2 
	$$g(x) = \sqrt x \cdot sin(x)$$
	$$g(x) = x^\frac{1}{2} \cdot sin(x)$$
	$$g'(x) = \frac{1}{2}x^\frac{-1}{2} \cdot sin(x) + x^\frac{1}{2} \cdot cos(x)$$
	$$g'(x) = \frac{\sqrt{x}(sin(x)+2x\cdot cos(x))}{2x}$$
## Ex. 3 
	$$g(x) = sin(x)x^2$$
	$$g'(x) = cos(x)x^2 + sin(x)2x$$
	$$g'(x) = \frac{1}{2}x^\frac{-1}{2} \cdot sin(x) + x^\frac{1}{2} \cdot cos(x)$$
	$$g'(x) = \frac{\sqrt{x}(sin(x)+2x\cdot cos(x))}{2x}$$
# Regra do Quociente
$$(\frac{v}{u}​)'= \frac{u'v + uv'}{v^2}​$$